test/EqB.fst
@@ -1,14 +1,24 @@
 module EqB
 
+open FStar.HyperStack.ST
+
 open FStar.Buffer
 
-let main () =
+let main (): St Int32.t =
+  push_frame ();
   let b1 = createL [ 1; 2; 3 ] in
   let b2 = createL [ 1; 3; 3 ] in
   let b3 = createL [ 1; 2; 3 ] in
   let b4 = createL [ [ 1; 2 ] ] in
   let b5 = createL [ [ 1; 2 ] ] in
-  if eqb b1 b3 3ul && not (eqb b2 b3 3ul) && eqb b4 b5 1ul then
-    0l
-  else
-    1l
+  let t1 = eqb b1 b3 3ul in
+  let t2 = not (eqb b2 b3 3ul) in
+  let t3 = eqb b4 b5 1ul in
+  let r =
+    if t1 && t2 && t3 then
+      0l
+    else
+      1l
+  in
+  pop_frame ();
+  r
