test/RecursivePoly.fst
@@ -7,6 +7,8 @@ module B = FStar.Buffer
 type pointer (t: Type0) =
   b:B.buffer t { B.length b = 1 }
 
+#set-options "--__no_positivity"
+noeq
 type linked_list (a: Type0) =
   | Null
   | Cons: elt:a -> next:pointer (linked_list a) -> linked_list a
@@ -18,4 +20,4 @@ let g (x: linked_list FStar.UInt64.t): Stack unit (fun _ -> true) (fun _ _ _ -> 
   ()
 
 let main () =
-  C.exit_success
+  C.EXIT_SUCCESS
